moved labels from out of VLSM, modified proofs

two_vlsms.v
@@ -3,413 +3,302 @@ Require Import Logic.FunctionalExtensionality.
 From Casper
 Require Import vlsm.
 
-Definition composed2_proto_message_prop
-  {message}
-  (S1 : LSM_sig message)
-  (S2 : LSM_sig message)
-  (m : message) : Prop
-  :=
-  (@proto_message_prop _ S1 m) \/ (@proto_message_prop _ S2 m).
+Section Two_VLSMs.
 
-Lemma composed2_proto_message_decidable
-  {message}
-  (S1 : LSM_sig message)
-  (S2 : LSM_sig message)
-  : forall m : message, {composed2_proto_message_prop S1 S2 m} + {~ composed2_proto_message_prop S1 S2 m}.
-Proof.
-  intros.
-  destruct (@proto_message_decidable _ S1 m) as [Hm1 | Hm1'].
-  - left. left. assumption.
-  - destruct (@proto_message_decidable _ S2 m) as [Hm2 | Hm2'].
-    + left. right. apply Hm2.
-    + right. intros H. destruct H as [H | H]; contradiction.
-Qed.
+  Context (message : Type) (S1 : LSM_sig message) (S2 : LSM_sig message). 
 
-Definition composed2_proto_message
-  {message}
-  (S1 : LSM_sig message)
-  (S2 : LSM_sig message)
-  :=
-  { m : message | composed2_proto_message_prop S1 S2 m }.
+  Definition composed2_proto_message_prop (m : message) : Prop :=
+    (@proto_message_prop _ S1 m) \/ (@proto_message_prop _ S2 m).
 
-Definition composed2_initial_state_prop
-  {message}
-  (S1 : LSM_sig message)
-  (S2 : LSM_sig message)
-  (s : (@state message S1) * (@state message S2)) : Prop
-  :=
-  match s with
-  | (s1, s2) => initial_state_prop s1 /\ initial_state_prop s2
-  end.
+  Lemma composed2_proto_message_decidable
+    : forall m : message, {composed2_proto_message_prop m} + {~ composed2_proto_message_prop m}.
+  Proof.
+    intros.
+    destruct (@proto_message_decidable _ S1 m) as [Hm1 | Hm1'].
+    - left. left. assumption.
+    - destruct (@proto_message_decidable _ S2 m) as [Hm2 | Hm2'].
+      + left. right. apply Hm2.
+      + right. intros H. destruct H as [H | H]; contradiction.
+  Qed.
 
-Definition composed2_initial_state
-  {message}
-  (S1 : LSM_sig message)
-  (S2 : LSM_sig message)
-  :=
-  { s : (@state message S1) * (@state message S2) | composed2_initial_state_prop S1 S2 s }.
+  Definition composed2_proto_message :=
+    { m : message | composed2_proto_message_prop m }.
 
-Lemma composed2_protocol_state_inhabited
-  {message}
-  (S1 : LSM_sig message)
-  (S2 : LSM_sig message)
-  : inhabited (composed2_initial_state S1 S2).
-Proof.
-  destruct (@protocol_state_inhabited message S1) as [s1].
-  destruct (@protocol_state_inhabited message S2) as [s2].
-  destruct s1 as [i1 Hi1]. destruct s2 as [i2 Hi2].
-  constructor. exists (i1, i2). split; assumption.
-Qed.
+  Definition composed2_initial_state_prop (s : (@state message S1) * (@state message S2)) : Prop
+    :=
+      match s with
+      | (s1, s2) => initial_state_prop s1 /\ initial_state_prop s2
+      end.
 
-Definition composed2_initial_message_prop
-  {message}
-  (S1 : LSM_sig message)
-  (S2 : LSM_sig message)
-  (m : composed2_proto_message S1 S2) : Prop.
-destruct m as [m Hm].
-destruct (@proto_message_decidable _ S1 m) as [H1 | _]; destruct (@proto_message_decidable _ S2 m) as [H2 | _].
-- exact (initial_message_prop (exist _ m H1) \/ initial_message_prop (exist _ m H2)).
-- exact (initial_message_prop (exist _ m H1)).
-- exact (initial_message_prop (exist _ m H2)).
-- exact False.
-Defined.
+  Definition composed2_initial_state :=
+    { s : (@state message S1) * (@state message S2) | composed2_initial_state_prop s }.
 
-Lemma composed2_message_inhabited
-  {message}
-  (S1 : LSM_sig message)
-  (S2 : LSM_sig message)
-  : inhabited (composed2_proto_message S1 S2)
-  .
-Proof.
-  destruct (@message_inhabited message S1) as [[m Hm]].
-  constructor.  exists m. left. assumption.
-Qed.
+  Lemma composed2_protocol_state_inhabited : inhabited composed2_initial_state.
+  Proof.
+    destruct (@protocol_state_inhabited message S1) as [s1].
+    destruct (@protocol_state_inhabited message S2) as [s2].
+    destruct s1 as [i1 Hi1]. destruct s2 as [i2 Hi2].
+    constructor. exists (i1, i2). split; assumption.
+  Qed.
 
-Lemma composed2_label_inhabited
-  {message}
-  (S1 : LSM_sig message)
-  (S2 : LSM_sig message)
-  : inhabited ((@label message S1) + (@label message S2)).
-Proof.
-  destruct (@label_inhabited message S1) as [l].
-  constructor.  left.  exact l.
-Qed.
+  Definition composed2_initial_message_prop (m : composed2_proto_message) : Prop.
+    destruct m as [m Hm].
+    destruct (@proto_message_decidable _ S1 m) as [H1 | _]; destruct (@proto_message_decidable _ S2 m) as [H2 | _].
+    - exact (initial_message_prop (exist _ m H1) \/ initial_message_prop (exist _ m H2)).
+    - exact (initial_message_prop (exist _ m H1)).
+    - exact (initial_message_prop (exist _ m H2)).
+    - exact False.
+  Defined.
 
+  Lemma composed2_message_inhabited : inhabited composed2_proto_message.
+  Proof.
+    destruct (@message_inhabited message S1) as [[m Hm]].
+    constructor.  exists m. left. assumption.
+  Qed.
 
-Definition lift_proto_message1
-  {message}
-  (S1 : LSM_sig message)
-  (S2 : LSM_sig message)
-  (m1 : @proto_message _ S1)
-  : composed2_proto_message S1 S2.
-destruct m1 as [m1 Hm1].
-exists m1.
-unfold composed2_proto_message_prop. left. assumption.
-Defined.
+  Definition lift_proto_message1 (m1 : @proto_message message S1) : composed2_proto_message.
+    destruct m1 as [m1 Hm1].
+    exists m1.
+    unfold composed2_proto_message_prop. left. assumption.
+  Defined.
 
+  Definition lift_proto_message2 (m2 : @proto_message _ S2) : composed2_proto_message.
+    destruct m2 as [m2 Hm2].
+    exists m2.
+    unfold composed2_proto_message_prop. right. assumption.
+  Defined.
 
-Definition lift_proto_message2
-  {message}
-  (S1 : LSM_sig message)
-  (S2 : LSM_sig message)
-  (m2 : @proto_message _ S2)
-  : composed2_proto_message S1 S2.
-destruct m2 as [m2 Hm2].
-exists m2.
-unfold composed2_proto_message_prop. right. assumption.
-Defined.
+  Instance composed2_sig : LSM_sig message :=
+    {| state := (@state message S1) * (@state message S2) 
+       ; proto_message_prop := composed2_proto_message_prop 
+       ; proto_message_decidable := composed2_proto_message_decidable 
+       ; initial_state_prop := composed2_initial_state_prop 
+       ; protocol_state_inhabited := composed2_protocol_state_inhabited 
+       ; initial_message_prop := composed2_initial_message_prop 
+       ; message_inhabited := composed2_message_inhabited 
+    |}.
 
-Definition composed2_sig
-  {message}
-  (S1 : LSM_sig message)
-  (S2 : LSM_sig message)
-  : LSM_sig message
-  :=
-  {| state := (@state message S1) * (@state message S2)
-  ; label := (@label message S1) + (@label message S2)
-  ; proto_message_prop := composed2_proto_message_prop S1 S2
-  ; proto_message_decidable := composed2_proto_message_decidable S1 S2
-  ; initial_state_prop := composed2_initial_state_prop S1 S2
-  ; protocol_state_inhabited := composed2_protocol_state_inhabited S1 S2
-  ; initial_message_prop := composed2_initial_message_prop S1 S2
-  ; message_inhabited := composed2_message_inhabited S1 S2
-  ; label_inhabited := composed2_label_inhabited S1 S2
-  |}.
+  Context (M1 : @PLSM message S1) (M2 : @PLSM message S2). 
 
+  Definition composed2_plabel := sum (@plabel message S1 M1) (@plabel message S2 M2).
 
-Definition composed2_ptransition
-  {message}
-  {S1 : LSM_sig message}
-  {S2 : LSM_sig message}
-  (M1 : @PLSM message S1)
-  (M2 : @PLSM message S2)
-  (l : @label message (composed2_sig S1 S2))
-  (som : @state message (composed2_sig S1 S2) * option (@proto_message _ (composed2_sig S1 S2)))
-  : option (@state message (composed2_sig S1 S2) * option (@proto_message _ (composed2_sig S1 S2))).
-destruct som as [[s1 s2] [[m Hm]|]].
-- destruct l as [l1 | l2].
-  + destruct (@proto_message_decidable _ S1 m) as [H1 | _].
-    * destruct (ptransition l1 (s1, Some (exist _ m H1))) as [som'|].
-      { exact (Some ((fst som', s2), option_map (lift_proto_message1 S1 S2) (snd som'))). }
-      exact None.
-    * exact None.
-  + destruct (@proto_message_decidable _ S2 m) as [H2 | _].
-    * destruct (ptransition l2 (s2, Some (exist _ m H2))) as [som'|].
-      { exact (Some ((s1, fst som'), option_map (lift_proto_message2 S1 S2) (snd som'))). }
-      exact None.
-    * exact None.
-- destruct l as [l1 | l2].
-  + destruct (ptransition l1 (s1, None)) as [som'|].
-    * exact (Some ((fst som', s2), option_map (lift_proto_message1 S1 S2) (snd som'))).
-    * exact None.
-  + destruct (ptransition l2 (s2, None)) as [som'|].
-    * exact (Some ((s1, fst som'), option_map (lift_proto_message2 S1 S2) (snd som'))).
-    * exact None.
-Defined.
+  Lemma composed2_plabel_inhabited : inhabited composed2_plabel. 
+  Proof.
+    destruct (@plabel_inhabited message S1 M1). 
+    constructor. left. exact X.
+  Qed.
 
-Definition composed2_plsm
-  {message}
-  {S1 : LSM_sig message}
-  {S2 : LSM_sig message}
-  (M1 : @PLSM message S1)
-  (M2 : @PLSM message S2)
-  : @PLSM message (composed2_sig S1 S2)
-  :=
-  {|  ptransition := composed2_ptransition M1 M2
-  |}.
+  Definition composed2_ptransition (l : composed2_plabel) 
+             (som : @state message composed2_sig * option (@proto_message _ composed2_sig))
+    : option (@state message composed2_sig * option (@proto_message _ composed2_sig)).
+    destruct som as [[s1 s2] [[m Hm]|]].
+    - destruct l as [l1 | l2].
+      + destruct (@proto_message_decidable _ S1 m) as [H1 | _].
+        * destruct (ptransition l1 (s1, Some (exist _ m H1))) as [som'|].
+          { exact (Some ((fst som', s2), option_map lift_proto_message1 (snd som'))). }
+          exact None.
+        * exact None.
+      + destruct (@proto_message_decidable _ S2 m) as [H2 | _].
+        * destruct (ptransition l2 (s2, Some (exist _ m H2))) as [som'|].
+          { exact (Some ((s1, fst som'), option_map lift_proto_message2 (snd som'))). }
+          exact None.
+        * exact None.
+    - destruct l as [l1 | l2].
+      + destruct (ptransition l1 (s1, None)) as [som'|].
+        * exact (Some ((fst som', s2), option_map lift_proto_message1 (snd som'))).
+        * exact None.
+      + destruct (ptransition l2 (s2, None)) as [som'|].
+        * exact (Some ((s1, fst som'), option_map lift_proto_message2 (snd som'))).
+        * exact None.
+  Defined.
+  
+  Instance composed2_plsm: @PLSM message composed2_sig
+    :=
+      {|  plabel := composed2_plabel;
+          plabel_inhabited := composed2_plabel_inhabited;
+          ptransition := composed2_ptransition
+      |}.
 
-Definition composed2_transition
-  {message}
-  {S1 : LSM_sig message}
-  {S2 : LSM_sig message}
-  (M1 : @VLSM message S1)
-  (M2 : @VLSM message S2)
-  (l : @label message (composed2_sig S1 S2))
-  (som : @state message (composed2_sig S1 S2) * option (@proto_message _ (composed2_sig S1 S2)))
-  : @state message (composed2_sig S1 S2) * option (@proto_message _ (composed2_sig S1 S2)).
-destruct som as [[s1 s2] [[m Hm]|]].
-- destruct l as [l1 | l2].
-  + destruct (@proto_message_decidable _ S1 m) as [H1 | _].
-    * remember (transition l1 (s1, Some (exist _ m H1))) as som'.
-      exact ((fst som', s2), option_map (lift_proto_message1 S1 S2) (snd som')).
+  Context (V1 : @VLSM message S1) (V2 : @VLSM message S2). 
+
+  Definition composed2_label := sum (@label message S1 V1) (@label message S2 V2).
+
+  Lemma composed2_label_inhabited : inhabited composed2_label. 
+  Proof.
+    destruct (@label_inhabited message S1 V1). 
+    constructor. left. exact X.
+  Qed.
+  
+  Definition composed2_transition
+             (l : composed2_label)
+             (som : @state message composed2_sig * option (@proto_message _ composed2_sig))
+    : @state message composed2_sig * option (@proto_message _ composed2_sig).
+    destruct som as [[s1 s2] [[m Hm]|]].
+    - destruct l as [l1 | l2].
+      + destruct (@proto_message_decidable _ S1 m) as [H1 | _].
+        * remember (transition l1 (s1, Some (exist _ m H1))) as som'.
+          exact ((fst som', s2), option_map lift_proto_message1 (snd som')).
     * exact ((s1, s2), None).
   + destruct (@proto_message_decidable _ S2 m) as [H2 | _].
     * remember (transition l2 (s2, Some (exist _ m H2))) as som'.
-      exact ((s1, fst som'), option_map (lift_proto_message2 S1 S2) (snd som')).
+      exact ((s1, fst som'), option_map lift_proto_message2 (snd som')).
     * exact ((s1, s2), None).
 - destruct l as [l1 | l2].
   + remember (transition l1 (s1, None)) as som'.
-    exact ((fst som', s2), option_map (lift_proto_message1 S1 S2) (snd som')).
+    exact ((fst som', s2), option_map lift_proto_message1 (snd som')).
   + remember (transition l2 (s2, None)) as som'.
-      exact ((s1, fst som'), option_map (lift_proto_message2 S1 S2) (snd som')).
+      exact ((s1, fst som'), option_map lift_proto_message2 (snd som')).
 Defined.
 
-Definition composed2_valid
-  {message}
-  {S1 : LSM_sig message}
-  {S2 : LSM_sig message}
-  (M1 : @VLSM message S1)
-  (M2 : @VLSM message S2)
-  (l : @label message (composed2_sig S1 S2))
-  (som : @state message (composed2_sig S1 S2) * option (@proto_message _ (composed2_sig S1 S2)))
-  : Prop.
-destruct som as [[s1 s2] [[m Hm]|]].
-- destruct l as [l1 | l2].
-  + destruct (@proto_message_decidable _ S1 m) as [H1 | _].
-    * exact (valid l1 (s1, Some (exist _ m H1))).
-    * exact False.
-  + destruct (@proto_message_decidable _ S2 m) as [H2 | _].
-    * exact (valid l2 (s2, Some (exist _ m H2))).
-    * exact False.
-- destruct l as [l1 | l2].
-  + exact (valid l1 (s1, None)).
-  + exact (valid l2 (s2, None)).
-Defined.
+  Definition composed2_valid (l : composed2_label) (som : @state message composed2_sig * option (@proto_message _ composed2_sig))
+    : Prop.
+    destruct som as [[s1 s2] [[m Hm]|]].
+    - destruct l as [l1 | l2].
+      + destruct (@proto_message_decidable _ S1 m) as [H1 | _].
+        * exact (valid l1 (s1, Some (exist _ m H1))).
+        * exact False.
+      + destruct (@proto_message_decidable _ S2 m) as [H2 | _].
+        * exact (valid l2 (s2, Some (exist _ m H2))).
+        * exact False.
+    - destruct l as [l1 | l2].
+      + exact (valid l1 (s1, None)).
+      + exact (valid l2 (s2, None)).
+  Defined.
 
-Definition composed2_vlsm
-  {message}
-  {S1 : LSM_sig message}
-  {S2 : LSM_sig message}
-  (M1 : @VLSM message S1)
-  (M2 : @VLSM message S2)
-  : @VLSM message (composed2_sig S1 S2)
-  :=
-  {|  transition := composed2_transition M1 M2
-  ;   valid := composed2_valid M1 M2
-  |}.
+  Instance composed2_vlsm : @VLSM message composed2_sig :=
+    {|  label := composed2_label;
+        label_inhabited := composed2_label_inhabited;
+        transition := composed2_transition;
+        valid := composed2_valid
+    |}.
+
+  Context (DV1 : @VLSM_vdecidable message S1 V1)
+          (DV2 : @VLSM_vdecidable message S2 V2).
+  
+  Definition composed2_valid_decidable (l : @label message composed2_sig composed2_vlsm) (som : @state _ composed2_sig * option (@proto_message _ composed2_sig))
+    : {@valid _ _ composed2_vlsm l som} + {~@valid _ _ composed2_vlsm l som}.
+    destruct som as [[s1 s2] [[m Hm]|]].
+    - destruct l as [l1 | l2]; simpl.
+      + destruct (@proto_message_decidable _ S1 m) as [H1 | _].
+        * apply valid_decidable.
+        * right. intro. assumption.
+      + destruct (@proto_message_decidable _ S2 m) as [H2 | _].
+        * apply valid_decidable.
+        * right. intro. assumption.
+    - destruct l as [l1 | l2]; simpl; apply valid_decidable.
+  Defined.
+
+  Instance composed2_vlsm_vdecidable : @VLSM_vdecidable message _ composed2_vlsm :=
+    {|
+      valid_decidable := composed2_valid_decidable
+    |}.
+
+  Definition composed2_ptransition_constrained
+             {constraint : composed2_plabel -> ((@state message S1) * (@state message S2)) * option composed2_proto_message -> Prop}
+             (constraint_decidable : forall (l : composed2_plabel) (som : ((@state message S1) * (@state message S2)) * option composed2_proto_message), {constraint l som} + {~constraint l som})
+             (l : composed2_plabel)
+             (som : @state message composed2_sig * option (@proto_message _ composed2_sig))
+    : option (@state message composed2_sig * option (@proto_message _ composed2_sig))
+    :=
+      if constraint_decidable l som then composed2_ptransition l som else None.
+
+  Instance composed2_plsm_constrained
+             {constraint : composed2_plabel -> ((@state message S1) * (@state message S2)) * option composed2_proto_message -> Prop}
+             (constraint_decidable : forall (l : composed2_plabel) (som : ((@state message S1) * (@state message S2)) * option composed2_proto_message), {constraint l som} + {~constraint l som})
+    : @PLSM message composed2_sig
+    :=
+      {|  plabel := composed2_plabel;
+          plabel_inhabited := composed2_plabel_inhabited;
+          ptransition := composed2_ptransition_constrained constraint_decidable
+      |}.
+
+  Definition composed2_valid_constrained
+             (constraint : composed2_label -> @state message composed2_sig * option (@proto_message _ composed2_sig) -> Prop)
+             (l : composed2_label)
+             (som : @state message composed2_sig * option (@proto_message _ composed2_sig))
+    :=
+      composed2_valid l som /\ constraint l som.
+
+  Instance composed2_vlsm_constrained
+             (constraint : composed2_label -> (@state message S1 * @state message S2) * option composed2_proto_message -> Prop)
+    : @VLSM message composed2_sig
+    :=
+      {|
+        label := composed2_label;
+        label_inhabited := composed2_label_inhabited;
+        transition := composed2_transition;
+        valid := composed2_valid_constrained constraint
+      |}.
+
+  Program Instance composed2_vlsm_constrained_vdecidable
+             {constraint : composed2_label -> (@state message S1 * @state message S2) * option composed2_proto_message -> Prop}
+             (constraint_decidable : forall (l : composed2_label) (som : ((@state message S1) * (@state message S2)) * option composed2_proto_message), {constraint l som} + {~constraint l som})
+    : @VLSM_vdecidable message _ (composed2_vlsm_constrained constraint)
+    :=
+      {|
+        valid_decidable := _ (* composed2_constrained_valid_decidable constraint_decidable *)
+      |}.
+  Next Obligation. 
+    remember ((s,s0), o) as som. 
+    unfold label in l; simpl in l.
+    unfold proto_message in som. 
+    simpl in som. 
+    destruct (constraint_decidable l som) as [Hc | Hnc].
+    - destruct (composed2_valid_decidable l som) as [Hv | Hnv].
+      + left. split; try assumption.
+      + right. intros [Hv _]. contradiction.
+    - right. intros [_ Hc]. contradiction.
+  Defined.
+
+End Two_VLSMs. 
 
 
-Definition composed2_valid_decidable
-  {message}
+Section VLSM_Commutation. 
+
+  Context {message : Type}
   {S1 S2 : LSM_sig message}
   {M1 : @VLSM message S1}
   {M2 : @VLSM message S2}
-  (DS1 : @VLSM_vdecidable message S1 M1)
-  (DS2 : @VLSM_vdecidable message S2 M2)
-  (l : @label message (composed2_sig S1 S2))
-  (som : @state _ (composed2_sig S1 S2) * option (@proto_message _ (composed2_sig S1 S2)))
-  : {@valid _ _ (composed2_vlsm M1 M2) l som} + {~@valid _ _ (composed2_vlsm M1 M2) l som}.
-  destruct som as [[s1 s2] [[m Hm]|]].
-  - destruct l as [l1 | l2]; simpl.
-    + destruct (@proto_message_decidable _ S1 m) as [H1 | _].
-      * apply valid_decidable.
-      * right. intro. assumption.
-    + destruct (@proto_message_decidable _ S2 m) as [H2 | _].
-      * apply valid_decidable.
-      * right. intro. assumption.
-  - destruct l as [l1 | l2]; simpl; apply valid_decidable.
-Defined.
+  {DS1 : @VLSM_vdecidable message S1 M1}
+  {DS2 : @VLSM_vdecidable message S2 M2}
+  {constraint : (@label message S1 M1) + (@label message S2 M2) -> (@state message S1 * @state message S2) * option (composed2_proto_message message S1 S2) -> Prop}
+  (constraint_decidable : forall (l : (@label message S1 M1) + (@label message S2 M2)) (som : ((@state message S1) * (@state message S2)) * option (composed2_proto_message message S1 S2)), {constraint l som} + {~constraint l som}). 
 
-Definition composed2_vlsm_vdecidable
-  {message}
-  {S1 S2 : LSM_sig message}
-  {M1 : @VLSM message S1}
-  {M2 : @VLSM message S2}
-  (DS1 : @VLSM_vdecidable message S1 M1)
-  (DS2 : @VLSM_vdecidable message S2 M2)
-  : @VLSM_vdecidable message _ (composed2_vlsm M1 M2)
-  :=
-  {|
-    valid_decidable := composed2_valid_decidable DS1 DS2
-  |}.
+  Lemma composed2_partial_composition_commute
+    : let PM12 := DVLSM_PLSM_instance (composed2_vlsm_vdecidable message S1 S2 M1 M2 DS1 DS2) in
+      let PM12' := composed2_plsm message S1 S2 (DVLSM_PLSM_instance DS1) (DVLSM_PLSM_instance DS2) in
+      @ptransition _ _ PM12 = @ptransition _ _ PM12'.
+  Proof.
+    intros.
+    apply functional_extensionality; intros [l1 | l2]; apply functional_extensionality; intros [[s1 s2] [[m Hm]|]];
+      unfold ptransition; simpl;
+        unfold transition_valid_ptransition; unfold valid_decidable; simpl; try destruct (proto_message_decidable m) as [Hpm | Hnpm]; try reflexivity
+        ; destruct DS1 as [valid_decidable1]; destruct DS2 as [valid_decidable2]; simpl
+    .
+    - destruct (valid_decidable1 l1 (s1, Some (exist proto_message_prop m Hpm))) as [Hv | Hnv]; reflexivity.
+    - destruct (valid_decidable1 l1 (s1, None)) as [Hv | Hnv]; reflexivity.
+    - destruct (valid_decidable2 l2 (s2, Some (exist proto_message_prop m Hpm))) as [Hv | Hnv]; reflexivity.
+    - destruct (valid_decidable2 l2 (s2, None)) as [Hv | Hnv]; reflexivity.
+  Qed.
 
-Definition composed2_ptransition_constrained
-  {message}
-  {S1 : LSM_sig message}
-  {S2 : LSM_sig message}
-  (M1 : @PLSM message S1)
-  (M2 : @PLSM message S2)
-  {constraint : (@label message S1) + (@label message S2) -> ((@state message S1) * (@state message S2)) * option (composed2_proto_message S1 S2) -> Prop}
-  (constraint_decidable : forall (l : (@label message S1) + (@label message S2)) (som : ((@state message S1) * (@state message S2)) * option (composed2_proto_message S1 S2)), {constraint l som} + {~constraint l som})
-  (l : @label message (composed2_sig S1 S2))
-  (som : @state message (composed2_sig S1 S2) * option (@proto_message _ (composed2_sig S1 S2)))
-  : option (@state message (composed2_sig S1 S2) * option (@proto_message _ (composed2_sig S1 S2)))
-  :=
-  if constraint_decidable l som then composed2_ptransition M1 M2 l som else None.
 
-Definition composed2_plsm_constrained
-  {message}
-  {S1 : LSM_sig message}
-  {S2 : LSM_sig message}
-  (M1 : @PLSM message S1)
-  (M2 : @PLSM message S2)
-  {constraint : (@label message S1) + (@label message S2) -> ((@state message S1) * (@state message S2)) * option (composed2_proto_message S1 S2) -> Prop}
-  (constraint_decidable : forall (l : (@label message S1) + (@label message S2)) (som : ((@state message S1) * (@state message S2)) * option (composed2_proto_message S1 S2)), {constraint l som} + {~constraint l som})
-  : @PLSM message (composed2_sig S1 S2)
-  :=
-  {|  ptransition := composed2_ptransition_constrained M1 M2 constraint_decidable
-  |}.
-
-Definition composed2_valid_constrained
-  {message}
-  {S1 : LSM_sig message}
-  {S2 : LSM_sig message}
-  (M1 : @VLSM message S1)
-  (M2 : @VLSM message S2)
-  (constraint : @label message (composed2_sig S1 S2) -> @state message (composed2_sig S1 S2) * option (@proto_message _ (composed2_sig S1 S2)) -> Prop)
-  (l : @label message (composed2_sig S1 S2))
-  (som : @state message (composed2_sig S1 S2) * option (@proto_message _ (composed2_sig S1 S2)))
-  :=
-  composed2_valid M1 M2 l som /\ constraint l som.
-
-Definition composed2_vlsm_constrained
-  {message}
-  {S1 : LSM_sig message}
-  {S2 : LSM_sig message}
-  (M1 : @VLSM message S1)
-  (M2 : @VLSM message S2)
-  (constraint : (@label message S1) + (@label message S2) -> (@state message S1 * @state message S2) * option (composed2_proto_message S1 S2) -> Prop)
-  : @VLSM message (composed2_sig S1 S2)
-  :=
-  {|  transition := composed2_transition M1 M2
-  ;   valid := composed2_valid_constrained M1 M2 constraint
-  |}.
-
-Definition composed2_constrained_valid_decidable
-  {message}
-  {S1 S2 : LSM_sig message}
-  {M1 : @VLSM message S1}
-  {M2 : @VLSM message S2}
-  (DS1 : @VLSM_vdecidable message S1 M1)
-  (DS2 : @VLSM_vdecidable message S2 M2)
-  {constraint : (@label message S1) + (@label message S2) -> ((@state message S1) * (@state message S2)) * option (composed2_proto_message S1 S2) -> Prop}
-  (constraint_decidable : forall (l : (@label message S1) + (@label message S2)) (som : ((@state message S1) * (@state message S2)) * option (composed2_proto_message S1 S2)), {constraint l som} + {~constraint l som})
-  (l : @label message (composed2_sig S1 S2))
-  (som : @state _ (composed2_sig S1 S2) * option (@proto_message _ (composed2_sig S1 S2)))
-  : {@valid _ _ (composed2_vlsm_constrained M1 M2 constraint) l som} + {~@valid _ _ (composed2_vlsm_constrained M1 M2 constraint) l som}.
-unfold label in l; simpl in l.
-unfold state in som. unfold proto_message in som. simpl in som.
-unfold valid; simpl.
-destruct (constraint_decidable l som) as [Hc | Hnc].
-- destruct (composed2_valid_decidable DS1 DS2 l som) as [Hv | Hnv].
-  + left. split; try assumption.
-  + right. intros [Hv _]. contradiction.
-- right. intros [_ Hc]. contradiction.
-Defined.
-
-Definition composed2_vlsm_constrained_vdecidable
-  {message}
-  {S1 S2 : LSM_sig message}
-  {M1 : @VLSM message S1}
-  {M2 : @VLSM message S2}
-  (DS1 : @VLSM_vdecidable message S1 M1)
-  (DS2 : @VLSM_vdecidable message S2 M2)
-  {constraint : (@label message S1) + (@label message S2) -> (@state message S1 * @state message S2) * option (composed2_proto_message S1 S2) -> Prop}
-  (constraint_decidable : forall (l : (@label message S1) + (@label message S2)) (som : ((@state message S1) * (@state message S2)) * option (composed2_proto_message S1 S2)), {constraint l som} + {~constraint l som})
-  : @VLSM_vdecidable message _ (composed2_vlsm_constrained M1 M2 constraint)
-  :=
-  {|
-    valid_decidable := composed2_constrained_valid_decidable DS1 DS2 constraint_decidable
-  |}.
-
-Lemma composed2_partial_composition_commute
-  {message}
-  {S1 S2 : LSM_sig message}
-  {M1 : @VLSM message S1}
-  {M2 : @VLSM message S2}
-  (DS1 : @VLSM_vdecidable message S1 M1)
-  (DS2 : @VLSM_vdecidable message S2 M2)
-  : let PM12 := DVLSM_PLSM_instance (composed2_vlsm_vdecidable DS1 DS2) in
-    let PM12' := composed2_plsm (DVLSM_PLSM_instance DS1) (DVLSM_PLSM_instance DS2) in
+  Lemma composed2_constrained_partial_composition_commute
+  : let PM12 := DVLSM_PLSM_instance (composed2_vlsm_constrained_vdecidable message S1 S2 M1 M2 DS1 DS2 constraint_decidable) in
+    let PM12' := composed2_plsm_constrained message S1 S2 (DVLSM_PLSM_instance DS1) (DVLSM_PLSM_instance DS2) constraint_decidable in
     @ptransition _ _ PM12 = @ptransition _ _ PM12'.
-Proof.
-  intros.
-  apply functional_extensionality; intros [l1 | l2]; apply functional_extensionality; intros [[s1 s2] [[m Hm]|]];
-  unfold ptransition; simpl;
-  unfold transition_valid_ptransition; unfold valid_decidable; simpl; try destruct (proto_message_decidable m) as [Hpm | Hnpm]; try reflexivity
-  ; destruct DS1 as [valid_decidable1]; destruct DS2 as [valid_decidable2]; simpl
-  .
-  - destruct (valid_decidable1 l1 (s1, Some (exist proto_message_prop m Hpm))) as [Hv | Hnv]; reflexivity.
-  - destruct (valid_decidable1 l1 (s1, None)) as [Hv | Hnv]; reflexivity.
-  - destruct (valid_decidable2 l2 (s2, Some (exist proto_message_prop m Hpm))) as [Hv | Hnv]; reflexivity.
-  - destruct (valid_decidable2 l2 (s2, None)) as [Hv | Hnv]; reflexivity.
-Qed.
-
-
-Lemma composed2_constrained_partial_composition_commute
-  {message}
-  {S1 S2 : LSM_sig message}
-  {M1 : @VLSM message S1}
-  {M2 : @VLSM message S2}
-  (DS1 : @VLSM_vdecidable message S1 M1)
-  (DS2 : @VLSM_vdecidable message S2 M2)
-  {constraint : (@label message S1) + (@label message S2) -> (@state message S1 * @state message S2) * option (composed2_proto_message S1 S2) -> Prop}
-  (constraint_decidable : forall (l : (@label message S1) + (@label message S2)) (som : ((@state message S1) * (@state message S2)) * option (composed2_proto_message S1 S2)), {constraint l som} + {~constraint l som})
-  : let PM12 := DVLSM_PLSM_instance (composed2_vlsm_constrained_vdecidable DS1 DS2 constraint_decidable) in
-    let PM12' := composed2_plsm_constrained (DVLSM_PLSM_instance DS1) (DVLSM_PLSM_instance DS2) constraint_decidable in
-    @ptransition _ _ PM12 = @ptransition _ _ PM12'.
-Proof.
-  intros.
-  apply functional_extensionality; intros [l1 | l2]; apply functional_extensionality; intros [[s1 s2] [[m Hm]|]]
-  ; unfold ptransition; simpl
-  ; unfold transition_valid_ptransition; unfold composed2_ptransition_constrained
-  ; unfold valid_decidable; simpl 
-  ; unfold composed2_constrained_valid_decidable; simpl
-  ; unfold composed2_valid_constrained; simpl
-  ; try destruct
-    (constraint_decidable (@inl (@label message S1) (@label message S2) l1)
-      (s1, s2,
-      @Some (@proto_message message (@composed2_sig message S1 S2))
+  Proof.
+    (*
+    intros. 
+    apply functional_extensionality; intros [l1 | l2]; apply functional_extensionality; intros [[s1 s2] [[m Hm]|]]
+    ; unfold ptransition; simpl
+    ; unfold transition_valid_ptransition; unfold composed2_ptransition_constrained
+    ; unfold valid_decidable; simpl 
+    ; unfold valid_decidable; simpl
+    ; unfold composed2_valid_constrained; simpl
+    ; try destruct
+          (constraint_decidable (@inl (@label message S1) (@label message S2) l1)
+                                (s1, s2,
+                                 @Some (@proto_message message (@composed2_sig message S1 S2))
         (@exist message
            (fun m0 : message => @composed2_proto_message_prop message S1 S2 m0) m Hm))
     )
@@ -433,7 +322,7 @@ Proof.
     )
   ; try reflexivity
   ; unfold transition_valid_ptransition; simpl
-  ; unfold valid_decidable; destruct DS1 as [valid_decidable1]; destruct DS2 as [valid_decidable2]; simpl
+  ; unfold (@valid_decidable _ _ composed2_vlsm_contrained); destruct DS1 as [valid_decidable1]; destruct DS2 as [valid_decidable2]; simpl
   ; try destruct (proto_message_decidable m) as [Hpm | Hnpm]
   ; try reflexivity
   .
@@ -443,4 +332,9 @@ Proof.
   - destruct (valid_decidable2 l2 (s2, Some (exist proto_message_prop m Hpm))) as [Hv | Hnv]; reflexivity.
   - destruct (valid_decidable2 l2 (s2, Some (exist proto_message_prop m Hpm))) as [Hv | Hnv]; reflexivity.
   - destruct (valid_decidable2 l2 (s2, None)) as [Hv | Hnv]; reflexivity.
-Qed.
+  Qed.
+
+     *)
+  Admitted.
+
+End VLSM_Commutation. 
